Optimizations/Canonicalizations/ConditionalPhase.thy
@@ -37,17 +37,23 @@ optimization NegateConditionFlipBranches: "((!e) ? x : y) \<longmapsto> (e ? y :
 
 optimization DefaultTrueBranch: "(true ? x : y) \<longmapsto> x" .
 
+value DefaultTrueBranch_code
+
 optimization DefaultFalseBranch: "(false ? x : y) \<longmapsto> y" .
 
 optimization ConditionalEqualBranches: "(e ? x : x) \<longmapsto> x" .
 
 optimization condition_bounds_x: "((u < v) ? x : y) \<longmapsto> x 
-    when (stamp_under (stamp_expr u) (stamp_expr v) \<and> wf_stamp u \<and> wf_stamp v)"
-  using stamp_under_defn by fastforce
+    when (StampUnder u v && WellFormed u && WellFormed v)"
+  using stamp_under_defn
+  by (smt (verit, ccfv_SIG) BinaryExprE ConditionalExprE StampEvalThms.wf_stamp_def TermRewrites.wf_stamp_def le_expr_def)
+(* by fastforce *)
 
 optimization condition_bounds_y: "((u < v) ? x : y) \<longmapsto> y 
-    when (stamp_under (stamp_expr v) (stamp_expr u) \<and> wf_stamp u \<and> wf_stamp v)"
-  using stamp_under_defn_inverse by fastforce
+    when (StampUnder v u && WellFormed u && WellFormed v)"
+  using stamp_under_defn_inverse
+  by (smt (verit, ccfv_threshold) BinaryExprE ConditionalExprE StampEvalThms.wf_stamp_def TermRewrites.wf_stamp_def le_expr_def)
+  (* by fastforce *)
 
 (** Start of new proofs **)
 
@@ -56,26 +62,28 @@ lemma val_optimise_integer_test:
   assumes "\<exists>v. x = IntVal 32 v"
   shows "val[((x & (IntVal 32 1)) eq (IntVal 32 0)) ? (IntVal 32 0) : (IntVal 32 1)] = 
          val[x & IntVal 32 1]"
-  using assms apply auto
+  using assms apply auto[1]
   apply (metis (full_types) bool_to_val.simps(2) val_to_bool.simps(1))
   by (metis (mono_tags, lifting) and_one_eq bool_to_val.simps(1) even_iff_mod_2_eq_zero odd_iff_mod_2_eq_one val_to_bool.simps(1))
 
 optimization ConditionalEliminateKnownLess: "((x < y) ? x : y) \<longmapsto> x 
-                                 when (stamp_under (stamp_expr x) (stamp_expr y)
-                                      \<and> wf_stamp x \<and> wf_stamp y)"
-    using stamp_under_defn by fastforce
+                                 when (StampUnder x y &&
+                                       WellFormed x && WellFormed y)"
+  using stamp_under_defn
+  by (smt (verit, best) BinaryExprE ConditionalExprE StampEvalThms.wf_stamp_def TermRewrites.wf_stamp_def le_expr_def)
+  (* by fastforce *)
 
 (* Optimisations *)
 optimization ConditionalEqualIsRHS: "((x eq y) ? x : y) \<longmapsto> y"
-  apply auto
+  apply auto[1]
   by (smt (verit) Value.inject(1) bool_to_val.simps(2) bool_to_val_bin.simps evalDet 
       intval_equals.elims val_to_bool.elims(1))
 
 (* todo not sure if this is done properly *)
 optimization normalizeX: "((x eq const (IntVal 32 0)) ? 
                                 (const (IntVal 32 0)) : (const (IntVal 32 1))) \<longmapsto> x
-                                when (IRExpr_up x = 1) \<and> stamp_expr x = IntegerStamp b 0 1" 
-  apply auto
+                                when (UpMaskEquals x 1) && (IsStamp x (IntegerStamp 32 0 1))" 
+  apply auto[1]
   subgoal premises p for m p v xa
     proof -
       obtain xa where xa: "[m,p] \<turnstile> x \<mapsto> xa"
@@ -92,24 +100,24 @@ optimization normalizeX: "((x eq const (IntVal 32 0)) ?
       then show ?thesis
         using xa by auto
     qed
-  done
+    done
 
 (* todo not sure if this is done properly *)
 optimization normalizeX2: "((x eq (const (IntVal 32 1))) ? 
                                  (const (IntVal 32 1)) : (const (IntVal 32 0))) \<longmapsto> x
-                                 when (x = ConstantExpr (IntVal 32 0) | (x = ConstantExpr (IntVal 32 1)))" .
+                                 when IsBool x" .
 
 (* todo not sure if this is done properly *)
 optimization flipX: "((x eq (const (IntVal 32 0))) ? 
                            (const (IntVal 32 1)) : (const (IntVal 32 0))) \<longmapsto> 
                             x \<oplus> (const (IntVal 32 1))
-                            when (x = ConstantExpr (IntVal 32 0) | (x = ConstantExpr (IntVal 32 1)))" .
+                            when IsBool x" .
 
 (* todo not sure if this is done properly *)
 optimization flipX2: "((x eq (const (IntVal 32 1))) ? 
                             (const (IntVal 32 0)) : (const (IntVal 32 1))) \<longmapsto> 
                             x \<oplus> (const (IntVal 32 1))
-                            when (x = ConstantExpr (IntVal 32 0) | (x = ConstantExpr (IntVal 32 1)))" .
+                            when IsBool x" .
 
 lemma stamp_of_default:
   assumes "stamp_expr x = default_stamp"
@@ -122,14 +130,15 @@ optimization OptimiseIntegerTest:
      "(((x & (const (IntVal 32 1))) eq (const (IntVal 32 0))) ? 
       (const (IntVal 32 0)) : (const (IntVal 32 1))) \<longmapsto> 
        x & (const (IntVal 32 1))
-       when (stamp_expr x = default_stamp \<and> wf_stamp x)"
+       when (IsStamp x default_stamp && WellFormed x)"
   apply simp apply (rule impI; (rule allI)+; rule impI)
   subgoal premises eval for m p v
 proof -
   obtain xv where xv: "[m, p] \<turnstile> x \<mapsto> xv"
     using eval by fast
   then have x32: "\<exists>v. xv = IntVal 32 v"
-    using stamp_of_default eval by auto
+    using stamp_of_default eval
+    by (metis TermRewrites.wf_stamp_def valid_value_elims(3))
   obtain lhs where lhs: "[m, p] \<turnstile> exp[(((x & (const (IntVal 32 1))) eq (const (IntVal 32 0))) ? 
       (const (IntVal 32 0)) : (const (IntVal 32 1)))] \<mapsto> lhs"
     using eval(2) by auto
@@ -152,7 +161,7 @@ optimization opt_optimise_integer_test_2:
      "(((x & (const (IntVal 32 1))) eq (const (IntVal 32 0))) ? 
                    (const (IntVal 32 0)) : (const (IntVal 32 1))) \<longmapsto> 
                    x
-                   when (x = ConstantExpr (IntVal 32 0) | (x = ConstantExpr (IntVal 32 1)))" .
+                   when IsBool x" .
 
 (*
 optimization opt_conditional_eliminate_known_less: "((x < y) ? x : y) \<longmapsto> x 
