Optimizations/Canonicalizations/XorPhase.thy
@@ -57,14 +57,14 @@ lemma val_eliminate_redundant_false:
 lemma exp_xor_self_is_false:
  assumes "wf_stamp x \<and> stamp_expr x = default_stamp" 
  shows   "exp[x \<oplus> x] \<ge> exp[false]" 
-  using assms apply auto unfolding wf_stamp_def
+  using assms apply auto[1] unfolding wf_stamp_def
   by (smt (z3) validDefIntConst IntVal0 Value.inject(1) bool_to_val.simps(2) 
       constantAsStamp.simps(1) evalDet int_signed_value_bounds new_int.simps unfold_const 
       val_xor_self_is_false_2 valid_int valid_stamp.simps(1) valid_value.simps(1) wf_value_def)
 
 lemma exp_eliminate_redundant_false:
   shows "exp[x \<oplus> false] \<ge> exp[x]"
-  using val_eliminate_redundant_false apply auto
+  using val_eliminate_redundant_false apply auto[1]
   subgoal premises p for m p xa
     proof -
       obtain xa where xa: "[m, p] \<turnstile> x \<mapsto> xa"
